Added coqdoc. Reduction now becomes Reduces.

src/Phasers/Taskview.v
@@ -1,10 +1,21 @@
+(** * Registration modes *)
 
-Inductive regmode : Set:=
-  | SIGNAL_ONLY : regmode
-  | WAIT_ONLY : regmode
-  | SIGNAL_WAIT : regmode.
+(**
+  There are three registration modes:
+  - [SIGNAL_ONLY] for tasks that do not wait for others and produce signals;
+  - [WAIT_ONLY] for tasks that wait for others and do not produce signals;
+  - [SIGNAL_WAIT] for tasks that wait for others and produce signals.
+*)
 
-(** Defines a <= relation between registration modes. *)
+Inductive regmode := SIGNAL_ONLY | WAIT_ONLY | SIGNAL_WAIT.
+
+(**
+  The relation [r_le], notation <=, establishes an ordering among registration
+  modes. This relation plays a crutial role in the registration of tasks.
+  Tasks can only register tasks being spawned. Registration must follow the
+  Capability rule that states that the registration mode of the spawned task
+  cannot be greater than the spawner.
+*)
 
 Inductive r_le : regmode -> regmode -> Prop :=
   | r_le_so:
@@ -15,31 +26,13 @@ Inductive r_le : regmode -> regmode -> Prop :=
     forall m,
     r_le m SIGNAL_WAIT.
 
-Record taskview := TV {
-  signal_phase: nat;
-  wait_phase: nat;
-  mode: regmode
-}.
+Module Notations.
+  Infix "<=" := (r_le) : reg_scope.
+End Notations.
 
-Definition make := TV 0 0 SIGNAL_WAIT.
-
-(** Standard mutators. *)
-
-Definition set_mode (v:taskview) (m:regmode) := TV v.(signal_phase) v.(wait_phase) m.
-Definition set_signal_phase (v:taskview) (n:nat) := TV n (wait_phase v) (mode v).
-Definition set_wait_phase (v:taskview) (n:nat) := TV (signal_phase v) n (mode v).
-
-(** Signal operation on taskviews. *)
-
-Definition signal (v:taskview) :=
-match v.(mode) with
-| SIGNAL_ONLY => set_signal_phase v (S (signal_phase v))
-| _ => set_signal_phase v (S (wait_phase v))
-end.
-
-(** Wait operation on taskviews. *)
-
-Definition wait (v:taskview) := set_wait_phase v (S (wait_phase v)).
+(**
+  Two important notions used throught the formalization are wait-/signal-capabilities.
+*)
 
 Inductive WaitCap : regmode -> Prop :=
   | wait_cap_sw:
@@ -57,13 +50,72 @@ Inductive SignalCap : regmode -> Prop :=
 
 Hint Constructors SignalCap.
 
-Module Notations.
-  Infix "<=" := (r_le) : reg_scope.
-End Notations.
+(** * Taskviews *)
+
+(**
+  A taskview is the local view of a task over a phaser.
+  It records: the number of signals the task issued,
+  the number of waits the task issued, and the task's
+  registration mode.
+*)
+
+Record taskview := TV {
+  signal_phase: nat;
+  wait_phase: nat;
+  mode: regmode
+}.
+
+(**
+  When creating a phaser, the creator is the only task registered in that phaser.
+  The first taskview is initialized in [SIGNAL_WAIT] mode and accounts for zero signals
+  and zero waits.
+ *)
+
+Definition make := TV 0 0 SIGNAL_WAIT.
+
+(** We define the mutators of a taskview, although they are only used internally. *)
+
+Definition set_signal_phase v n := TV n (wait_phase v) (mode v).
+Definition set_wait_phase v n := TV (signal_phase v) n (mode v).
+Definition set_mode v m := TV (signal_phase v) (wait_phase v) m.
+
+(** 
+  The two available mutators of taskviews are signal and wait, defined following.
+  The semantics of signal depends on the
+  registration mode of the issuer: when the issuer is registered in signal-only mode,
+  a signal increments the signal phase; otherwise, the signal becomes sets the signal-phase
+  one phase ahead of the wait phase.
+*)
+
+Definition signal v :=
+match mode v with
+| SIGNAL_ONLY => set_signal_phase v (S (signal_phase v))
+| _ => set_signal_phase v (S (wait_phase v))
+end.
+
+(**
+  A task with wait capability must interleave a signal with an await.
+  Only the first signal is observed by other tasks, and consecutive signals are ignored until
+  another the task invokes a waits, which is why the signal phase in relation to the wait phase.
+  We postpone discussing the error-conditions of invoking signal and wait to
+  the presentation of the operational semantics of task view operations.
+*)
+
+(**
+  The wait operation increments the wait-phase. Altough the semantics of wait does not depends
+  on the registration mode, invoking wait should be guarded by a precondition that we postpone
+  its definition to the following section.
+*)
+
+Definition wait v := set_wait_phase v (S (wait_phase v)).
+
+(* begin hide *)
 
 Section Facts.
   Import Notations.
   Open Scope reg_scope.
+
+  (** The equality of registration mode is decidable. *)
 
   Lemma regmode_eq_dec:
     forall (m1 m2:regmode),
@@ -72,6 +124,11 @@ Section Facts.
     intros.
     destruct m1, m2; solve [ left; auto | right; intuition; inversion H]. 
   Qed.
+
+  (**
+   We can simplify an expression that sets the mode it already has.
+   This lemma also shows the correctness of [set_mode].
+   *)
   
   Lemma set_mode_ident:
     forall v,
@@ -79,6 +136,9 @@ Section Facts.
   Proof.
     intros; destruct v; trivial.
   Qed.
+
+  (** A property of correctness: [set_mode] preserves the signal phase. *)
+  
 
   Lemma set_mode_preserves_signal_phase:
     forall v r,
@@ -88,6 +148,8 @@ Section Facts.
     destruct v; auto.
   Qed.
 
+  (** A property of correctness: [set_mode] preserves the wait phase. *)
+
   Lemma set_mode_preserves_wait_phase:
     forall v r,
     wait_phase (set_mode v r) =  wait_phase v.
@@ -96,12 +158,16 @@ Section Facts.
     destruct v; auto.
   Qed.
 
+  (** The initial taskview is registered in [SIGNAL_WAIT] mode. *)
+
   Lemma make_mode:
     mode make = SIGNAL_WAIT.
   Proof.
     unfold make.
     auto.
   Qed.
+
+  (** The initial taskview accounts for zero signals. *)
 
   Lemma make_signal_phase:
     signal_phase make = 0.
@@ -110,12 +176,16 @@ Section Facts.
     auto.
   Qed.
 
+  (** The initial taskview accounts for zero waits. *)
+
   Lemma make_wait_phase:
     wait_phase make = 0.
   Proof.
     unfold make.
     auto.
   Qed.
+
+  (** Checking for the wait capability is a decidable property. *)
 
   Lemma wait_cap_dec:
     forall r,
@@ -345,7 +415,23 @@ Section Facts.
 End Facts.
 
 Module Semantics.
-  Inductive op := | SIGNAL | WAIT.
+
+(* end hide *)
+  
+  (** * Small-step operational semantics*)
+
+  (**
+  The operational semantics of taskviews defines a closed set of operations [op]
+  that can change taskviews, that is signal and  wait.
+  *)
+
+  Inductive op := SIGNAL | WAIT.
+
+  (**
+  The of these operations can actually be represented by an interpreter function
+  [eval] that given an operation and a taskview applies the appropried operation to the given
+  taskview.
+  *)
 
   Definition eval (o:op) :=
   match o with
@@ -353,25 +439,39 @@ Module Semantics.
   | WAIT => wait
   end.
 
-  Inductive Reduce (v:taskview) : op -> taskview -> Prop :=
-    | reduce_signal:
-      Reduce v SIGNAL (signal v)
-    | reduce_wait:
-      wait_phase v < signal_phase v ->
-      Reduce v WAIT (wait v).
+  (**
+  The operational semantics not only define a closed set of operations that
+  can operate on a value (here a taskview), but also the preconditions of each operation.
+  Contrary to [eval], relation [Reduces] defines a precondition
+  to [wait]: in order to issue a wait, the wait phase must be behind (smaller than)
+  the signal phase.
+  *)
 
-  Lemma reduce_spec:
+  Inductive Reduces v : op -> taskview -> Prop :=
+    | tv_reduces_signal:
+      Reduces v SIGNAL (signal v)
+    | tv_reduces_wait:
+      wait_phase v < signal_phase v ->
+      Reduces v WAIT (wait v).
+
+  (**
+  A trivial property we choose to highlight is that [Reduces]
+  performs an [eval] on the right-hand side.
+  *)
+
+  Lemma reduces_spec:
     forall v o v',
-    Reduce v o v' ->
+    Reduces v o v' ->
     v' = eval o v.
   Proof.
     intros.
     inversion H; subst; simpl; trivial.
   Qed.
 
-  Lemma reduce_rw_signal:
+(* begin hide *)
+  Lemma reduces_rw_signal:
     forall v v',
-    Reduce v SIGNAL v' ->
+    Reduces v SIGNAL v' ->
     v' = signal v.
   Proof.
     intros.
@@ -379,9 +479,9 @@ Module Semantics.
     trivial.
   Qed.
 
-  Lemma reduce_rw_wait:
+  Lemma reduces_rw_wait:
     forall v v',
-    Reduce v WAIT v' ->
+    Reduces v WAIT v' ->
     v' = wait v.
   Proof.
     intros.
@@ -399,15 +499,16 @@ Module Semantics.
     auto using signal_preserves_mode, wait_preserves_mode.
   Qed.
 
-  Lemma reduce_preserves_mode:
+  Lemma reduces_preserves_mode:
     forall v o v',
-    Reduce v o v' ->
+    Reduces v o v' ->
     mode v' = mode v.
   Proof.
     intros.
-    apply reduce_spec in H.
+    apply reduces_spec in H.
     subst.
     auto using eval_preserves_mode.
   Qed.
 
 End Semantics.
+(* end hide *)
